SeqExt.dfy
@@ -1,0 +1,13 @@
+include "../libraries/src/Collections/Sequences/Seq.dfy"
+
+module SeqExt {
+  import opened Seq
+
+  lemma LemmaToSetAdds<X>(xs: seq<X>, ys: seq<X>)
+    ensures ToSet(xs) + ToSet(ys) == ToSet(xs + ys)
+  {
+    reveal ToSet();
+    assert forall x :: x in (xs + ys) <==> (x in xs) || (x in ys);
+  }
+        
+}
